Prove a property for the Congress contract
This proves a concrete property about any Congress contract deployed to
a blockchain. More specifically, we show that the count of transactions
sent out by any Congress contract will always be less than or equal to
the total number of actions it has receive in "create proposal"
messages.
Thus, this property is stated only over the transactions going in and
out to the Congress contract.
To prove this, we reason over incoming and outgoing transactions, the
internal state of the congress and also the actions in the blockchain
queue.

src/Congress.v
@@ -1,12 +1,14 @@
 From Coq Require Import ZArith.
-From Coq Require Import Program.Basics.
 From Coq Require Import Morphisms.
-
+From Coq Require Import Psatz.
+From Coq Require Import Program.
+From Coq Require Import Permutation.
 From SmartContracts Require Import Blockchain.
 From SmartContracts Require Import Oak.
 From SmartContracts Require Import Monads.
 From SmartContracts Require Import Containers.
 From SmartContracts Require Import Automation.
+From SmartContracts Require Import Extras.
 From RecordUpdate Require Import RecordUpdate.
 From Coq Require Import List.
 
@@ -176,35 +178,35 @@ Definition receive
   let is_from_owner := (sender =? state.(owner))%address in
   let is_from_member := FMap.mem sender state.(members) in
   let without_actions := option_map (fun new_state => (new_state, [])) in
-  match is_from_owner, is_from_member, maybe_msg with
-  | true, _, Some (transfer_ownership new_owner) =>
+  match maybe_msg, is_from_owner, is_from_member with
+  | Some (transfer_ownership new_owner), true, _ =>
         Some (state<|owner := new_owner|>, [])
 
-  | true, _, Some (change_rules new_rules) =>
+  | Some (change_rules new_rules), true, _ =>
         if validate_rules new_rules then
             Some (state<|state_rules := new_rules|>, [])
         else
             None
 
-  | true, _, Some (add_member new_member) =>
+  | Some (add_member new_member), true, _ =>
         Some (state<|members ::= FMap.add new_member tt|>, [])
 
-  | true, _, Some (remove_member old_member) =>
+  | Some (remove_member old_member), true, _ =>
         Some (state<|members ::= FMap.remove old_member|>, [])
 
-  | _, true, Some (create_proposal actions) =>
+  | Some (create_proposal actions), _, true =>
         Some (add_proposal actions chain state, [])
 
-  | _, true, Some (vote_for_proposal pid) =>
+  | Some (vote_for_proposal pid), _, true =>
         without_actions (vote_on_proposal sender pid 1 state)
 
-  | _, true, Some (vote_against_proposal pid) =>
+  | Some (vote_against_proposal pid), _, true =>
         without_actions (vote_on_proposal sender pid (-1) state)
 
-  | _, true, Some (retract_vote pid) =>
+  | Some (retract_vote pid), _, true =>
         without_actions (do_retract_vote sender pid state)
 
-  | _, _, Some (finish_proposal pid) =>
+  | Some (finish_proposal pid), _, _ =>
         do_finish_proposal pid state chain
 
   | _, _, _ =>
@@ -359,15 +361,518 @@ Proof. repeat intro; solve_contract_proper. Qed.
 
 Definition contract : Contract Setup Msg State :=
   build_contract version init init_proper receive receive_proper.
+Section Theories.
+Local Open Scope nat.
+(* cacts = congress actions here *)
+Definition num_acts_created_in_proposals chain address :=
+  let extract tx :=
+      match tx_body tx with
+      | tx_call msg =>
+        match deserialize msg with
+        | Some (create_proposal acts) => length acts
+        | _ => 0
+        end
+      | _ => 0
+      end in
+  sumnat extract (incoming_txs chain address).
 
+Definition num_cacts_in_raw_state state :=
+  sumnat (fun '(k, v) => length (actions v)) (FMap.elements (proposals state)).
+
+Definition num_cacts_in_state chain address :=
+  match contract_state chain address >>= deserialize with
+  | Some state => num_cacts_in_raw_state state
+  | None => 0
+  end.
+
+Definition num_outgoing_acts l address :=
+  let extract a :=
+      if address_eqb (act_from a) address
+      then 1
+      else 0 in
+  sumnat extract l.
+
+Instance num_acts_created_in_proposals_proper :
+  Proper (ChainEquiv ==> eq ==> eq) num_acts_created_in_proposals.
+Proof.
+  now repeat intro; subst; unfold num_acts_created_in_proposals;
+    match goal with
+    | [H: ChainEquiv _ _ |- _] => rewrite H
+    end.
+Qed.
+
+Instance num_cacts_in_state_proper :
+  Proper (ChainEquiv ==> eq ==> eq) num_cacts_in_state.
+Proof.
+  now repeat intro; subst; unfold num_cacts_in_state;
+    match goal with
+    | [H: ChainEquiv _ _ |- _] => rewrite H
+    end.
+Qed.
+
+Lemma num_outgoing_acts_app q1 q2 address :
+  num_outgoing_acts (q1 ++ q2) address =
+  num_outgoing_acts q1 address +
+  num_outgoing_acts q2 address.
+Proof.
+  unfold num_outgoing_acts.
+  now rewrite sumnat_app.
+Qed.
+
+Lemma num_outgoing_acts_block l contract :
+  address_is_contract contract = true ->
+  Forall ActIsFromAccount l ->
+  num_outgoing_acts l contract = 0.
+Proof.
+  intros is_contract all.
+  induction all; auto.
+  cbn in *.
+  destruct_address_eq; try congruence.
+  fold (num_outgoing_acts l contract); auto.
+Qed.
+
+Lemma num_outgoing_acts_call l contract :
+  num_outgoing_acts (map (build_act contract) l) contract = length l.
+Proof.
+  induction l; auto.
+  cbn.
+  destruct_address_eq; auto; congruence.
+Qed.
+
+Lemma num_outgoing_acts_call_ne to l contract :
+  to <> contract ->
+  num_outgoing_acts (map (build_act to) l) contract = 0.
+Proof.
+  intros neq.
+  induction l; auto.
+  cbn.
+  destruct_address_eq; auto; congruence.
+Qed.
+
+Lemma num_cacts_in_state_deployment (init_env : Environment) ctx setup state contract :
+  wc_init Congress.contract init_env ctx setup = Some state ->
+  num_cacts_in_state
+    (set_contract_state
+       contract state
+       (add_contract
+          contract Congress.contract init_env)) contract = 0.
+Proof.
+  intros init.
+  unfold num_cacts_in_state.
+  cbn.
+  unfold set_chain_contract_state.
+  destruct_address_eq; try congruence.
+  cbn in *.
+  destruct (deserialize setup); cbn in *; try congruence.
+  destruct (Congress.init _ _ _) eqn:congress_init; cbn in *; try congruence.
+  inversion init.
+  rewrite deserialize_serialize.
+  unfold Congress.init in congress_init.
+  destruct (validate_rules _); try congruence.
+  now inversion congress_init.
+Qed.
+
+Ltac remember_new_proposal :=
+  match goal with
+  | [|- context[FMap.add _ ?p]] => remember p as new_proposal
+  end.
+
+Lemma add_proposal_cacts cacts chain state :
+  num_cacts_in_raw_state (add_proposal cacts chain state) <=
+  num_cacts_in_raw_state state + length cacts.
+Proof.
+  unfold add_proposal, num_cacts_in_raw_state, constructor.
+  cbn.
+  destruct (FMap.find (next_proposal_id state) (proposals state)) as [proposal|] eqn:find.
+  - remember_new_proposal.
+    rewrite <- (FMap.add_remove _ (next_proposal_id state) new_proposal).
+    Hint Resolve FMap.find_remove.
+    rewrite <- (FMap.add_id _ _ _ find) at 2.
+    rewrite <- (FMap.add_remove _ (next_proposal_id state) proposal).
+    repeat rewrite FMap.elements_add; auto.
+    subst.
+    cbn.
+    lia.
+  - rewrite FMap.elements_add; auto.
+    cbn.
+    lia.
+Qed.
+
+Lemma vote_on_proposal_cacts_preserved addr pid vote_val state new_state :
+  vote_on_proposal addr pid vote_val state = Some new_state ->
+  num_cacts_in_raw_state new_state = num_cacts_in_raw_state state.
+Proof.
+  intros vote.
+  unfold vote_on_proposal in vote.
+  destruct (FMap.find _ _) eqn:found; cbn in *; try congruence.
+  inversion vote.
+  unfold num_cacts_in_raw_state.
+  cbn.
+  remember_new_proposal.
+  rewrite <- (FMap.add_id (proposals state) pid p) at 2; auto.
+  rewrite <- (FMap.add_remove _ pid p).
+  rewrite <- (FMap.add_remove _ pid new_proposal).
+  repeat rewrite FMap.elements_add; try apply FMap.find_remove.
+  subst; reflexivity.
+Qed.
+
+Lemma do_retract_vote_cacts_preserved addr pid state new_state :
+  do_retract_vote addr pid state = Some new_state ->
+  num_cacts_in_raw_state new_state = num_cacts_in_raw_state state.
+Proof.
+  intros retract.
+  unfold do_retract_vote in retract.
+  destruct (FMap.find _ _) eqn:found; cbn in *; try congruence.
+  destruct (FMap.find addr _); cbn in *; try congruence.
+  inversion retract.
+  unfold num_cacts_in_raw_state.
+  cbn.
+  remember_new_proposal.
+  rewrite <- (FMap.add_id (proposals state) pid p) at 2; auto.
+  rewrite <- (FMap.add_remove _ pid p).
+  rewrite <- (FMap.add_remove _ pid new_proposal).
+  Hint Resolve FMap.find_remove.
+  repeat rewrite FMap.elements_add; auto.
+  subst; reflexivity.
+Qed.
+
+Lemma remove_proposal_cacts pid state proposal :
+  FMap.find pid (proposals state) = Some proposal ->
+  num_cacts_in_raw_state (state <| proposals ::= FMap.remove pid |>) +
+  length (actions proposal) = num_cacts_in_raw_state state.
+Proof.
+  intros find.
+  unfold num_cacts_in_raw_state.
+  cbn.
+  rewrite <- (FMap.add_id (proposals state) pid proposal) at 2; auto.
+  rewrite <- FMap.add_remove.
+  rewrite FMap.elements_add; auto.
+  cbn.
+  lia.
+Qed.
+
+(* The next lemma shows that when we send out transactions, the
+state change will make up for number of outgoing actions queued. *)
+Lemma receive_state_well_behaved
+      chain ctx state msg new_state resp_acts :
+  receive chain ctx state msg = Some (new_state, resp_acts) ->
+  num_cacts_in_raw_state new_state + length resp_acts <=
+  num_cacts_in_raw_state state +
+  match msg with
+  | Some (create_proposal ls) => length ls
+  | _ => 0
+  end.
+Proof.
+  intros receive.
+  destruct msg as [msg|]; cbn in *; try congruence.
+  destruct msg; cbn in *; try congruence.
+  - (* transfer_ownership *)
+    destruct_address_eq; try congruence.
+    inversion receive; auto.
+  - (* change_rules *)
+    destruct_address_eq; cbn in *; destruct (validate_rules r); inversion receive; auto.
+  - (* add_member *)
+    destruct_address_eq; cbn in *; inversion receive; auto.
+  - (* remove_member *)
+    destruct_address_eq; cbn in *; inversion receive; auto.
+  - (* create_proposal *)
+    destruct (FMap.mem _ _); inversion receive.
+    cbn.
+    rewrite <- plus_n_O.
+    apply add_proposal_cacts.
+  - (* vote_for_proposal *)
+    destruct (FMap.mem _ _); try congruence.
+    destruct (vote_on_proposal _ _ _ _) eqn:vote; cbn in *; try congruence.
+    inversion receive; subst.
+    erewrite vote_on_proposal_cacts_preserved; eauto.
+  - (* vote_against_proposal *)
+    destruct (FMap.mem _ _); try congruence.
+    destruct (vote_on_proposal _ _ _ _) eqn:vote; cbn in *; try congruence.
+    inversion receive; subst.
+    erewrite vote_on_proposal_cacts_preserved; eauto.
+  - (* retract_vote *)
+    destruct (FMap.mem _ _); try congruence.
+    destruct (do_retract_vote _ _ _) eqn:retract; cbn in *; try congruence.
+    inversion receive; subst.
+    erewrite do_retract_vote_cacts_preserved; eauto.
+  - (* finish_proposal *)
+    unfold do_finish_proposal in receive.
+    destruct (FMap.find _ _) eqn:found; cbn in *; try congruence.
+    match goal with
+    | [H: (if ?a then _ else _) = Some _ |- _] => destruct a
+    end; cbn in *; try congruence.
+    inversion receive.
+    rewrite <- (remove_proposal_cacts _ _ _ found), map_length.
+    match goal with
+    | [|- context[if ?large_annoying_expression_i_should_refactor then _ else _]] =>
+      destruct large_annoying_expression_i_should_refactor
+    end; cbn.
+    + (* I wonder why these asserts are necessary... *)
+      assert (forall a b, a + b <= a + b + 0) by (intros; lia); auto.
+    + assert (forall a b, a + 0 <= a + b + 0) by (intros; lia); auto.
+Qed.
+
+(* This is the bookkeeping that does the serialization/deserialization
+for wc_receive. We should abstract this away. *)
+Lemma wc_receive_state_well_behaved
+      prev tx from contract amount msg ctx state new_state resp_acts :
+  let with_tx := add_tx tx prev in
+  tx = build_tx from contract amount (match msg with
+                                        | Some msg => tx_call msg
+                                        | None => tx_empty
+                                      end) ->
+  contract_state prev contract = Some state ->
+  wc_receive
+    Congress.contract
+    with_tx
+    ctx state msg = Some (new_state, resp_acts) ->
+  num_cacts_in_state
+    (set_contract_state contract new_state with_tx)
+    contract +
+  length resp_acts +
+  num_acts_created_in_proposals prev contract <=
+  num_cacts_in_state with_tx contract +
+  num_acts_created_in_proposals with_tx contract.
+Proof.
+  cbn zeta.
+  intros tx_eq prev_state_eq receive.
+  cbn -[Congress.receive add_tx] in receive.
+  destruct (deserialize state) eqn:deserialize_state; [|cbn in *; congruence].
+  destruct msg as [msg|]; [|cbn in *; congruence].
+  destruct (deserialize msg) eqn:deserialize_msg; [|cbn in *; congruence].
+  cbn -[Congress.receive add_tx] in receive.
+  destruct (Congress.receive _ _ _ _)
+    as [[new_state' resp_acts']|] eqn:congress_receive;
+    [|cbn in *; congruence].
+  cbn in receive.
+  inversion receive; subst new_state resp_acts.
+  unfold num_cacts_in_state.
+  cbn -[add_tx].
+  unfold set_chain_contract_state.
+  destruct_address_eq; try congruence.
+  cbn -[add_tx].
+  replace (contract_state (add_tx tx prev) contract) with (Some state) by auto.
+  cbn -[add_tx].
+  rewrite deserialize_state, deserialize_serialize.
+  unfold num_acts_created_in_proposals at 2.
+  cbn.
+  unfold add_tx_to_map.
+  destruct_address_eq; [|subst; cbn in *; congruence].
+  cbn.
+  fold (num_acts_created_in_proposals prev contract).
+  replace (tx_body tx) with (tx_call msg) by (subst; auto).
+  rewrite deserialize_msg.
+  pose proof (receive_state_well_behaved _ _ _ _ _ _ congress_receive).
+  lia.
+Qed.
+
+Lemma undeployed_contract_no_out_queue_count contract (state : ChainState) :
+  inhabited (ChainTrace empty_state state) ->
+  address_is_contract contract = true ->
+  env_contracts state contract = None ->
+  num_outgoing_acts (chain_state_queue state) contract = 0.
+Proof.
+  intros [trace] is_contract undeployed.
+  pose proof undeployed_contract_no_out_queue as all; specialize_hypotheses.
+  induction all; auto.
+  cbn.
+  match goal with
+  | [H: _ |- _] => now rewrite H; auto
+  end.
+Qed.
+
+Lemma undeployed_contract_not_from_self contract (state : ChainState) act acts :
+  inhabited (ChainTrace empty_state state) ->
+  address_is_contract contract = true ->
+  env_contracts state contract = None ->
+  chain_state_queue state = act :: acts ->
+  act_from act <> contract.
+Proof.
+  intros trace is_contract no_contract_prev queue_eq.
+  pose proof (
+         undeployed_contract_no_out_queue
+           _ _ trace is_contract no_contract_prev) as all.
+  rewrite queue_eq in *.
+  inversion all.
+  cbn in *.
+  destruct_address_eq; congruence.
+Qed.
+Hint Resolve undeployed_contract_no_out_queue_count : core.
+
+Arguments num_acts_created_in_proposals : simpl never.
+Arguments num_cacts_in_raw_state : simpl never.
+Arguments num_cacts_in_state : simpl never.
+Arguments num_outgoing_acts !l.
+
+Local Ltac rewrite_queues :=
+  repeat
+    match goal with
+    | [H: chain_state_queue _ = _ |- _] => rewrite H in *
+    end.
+
+Local Ltac solve_single :=
+  solve [
+      subst; auto;
+      cbn in *;
+      unfold add_tx_to_map, num_cacts_in_state, num_acts_created_in_proposals, num_outgoing_acts;
+      unfold set_chain_contract_state;
+      cbn in *;
+      subst; auto;
+      destruct_address_eq;
+      subst; auto;
+      cbn in *;
+      congruence].
+
+Local Ltac simpl_goal_invariant :=
+  repeat
+    match goal with
+    | [|- context G[outgoing_txs (env_chain (add_tx ?tx ?env)) ?addr]] =>
+      let new_goal := context G[tx :: outgoing_txs env addr] in
+      replace _ with new_goal by solve_single
+    | [|- context G[add_new_block_header _ _ ?env]] =>
+      let new_goal := context G[env] in
+      replace _ with new_goal by solve_single
+    | [|- context G[add_tx _ ?env]] =>
+      let new_goal := context G[env] in
+      replace _ with new_goal by solve_single
+    | [|- context G[set_contract_state _ _ ?env]] =>
+      let new_goal := context G[env] in
+      replace _ with new_goal by solve_single
+    | [|- context G[add_contract _ _ ?env]] =>
+      let new_goal := context G[env] in
+      replace _ with new_goal by solve_single
+    | [|- context G[num_outgoing_acts (?a ++ ?b) _]] =>
+      rewrite num_outgoing_acts_app
+    end.
+
+Local Ltac simpl_hyp_invariant :=
+  repeat
+    match goal with
+    | [IH: context[num_outgoing_acts (?act :: ?acts) ?addr] |- _] =>
+      replace (num_outgoing_acts (act :: acts) addr)
+        with (S (num_outgoing_acts acts addr))
+        in IH
+        by solve_single
+    | [IH: context[num_outgoing_acts (?act :: ?acts) ?addr] |- _] =>
+      replace (num_outgoing_acts (act :: acts) addr)
+        with (num_outgoing_acts acts addr)
+        in IH
+        by solve_single
+    end.
+
+Theorem congress_txs_well_behaved to contract :
+  inhabited (ChainTrace empty_state to) ->
+  env_contracts to contract = Some (Congress.contract : WeakContract) ->
+  num_cacts_in_state to contract + length (outgoing_txs to contract) +
+  num_outgoing_acts (chain_state_queue to) contract <=
+  num_acts_created_in_proposals to contract.
+Proof.
+  intros [trace] congress_deployed.
+  Hint Resolve contract_addr_format.
+  assert (address_is_contract contract = true) as addr_format by eauto.
+  remember empty_state eqn:eq.
+  (* Contract cannot have been deployed in empty trace so we solve that immediately. *)
+  induction trace as [|? ? ? evts IH evt]; subst; try solve_by_inversion.
+  destruct_chain_event; [|invert_chain_step|];
+    rewrite_queues;
+    repeat
+      match goal with
+      | [x := ?a : _ |- _] => pose proof (eq_refl : x = a); clearbody x
+      end.
+  - (* New block added, does not change any of the values *)
+    (* so basically just use IH directly. *)
+    rewrite_environment_equiv.
+    specialize_hypotheses.
+    simpl_goal_invariant.
+    rewrite num_outgoing_acts_block; auto.
+  - (* Transfer step: cannot be to contract, but can come from contract. *)
+    rewrite_environment_equiv.
+    specialize_hypotheses.
+    subst new_acts.
+    (* Handle from contract and not from contract separately. *)
+    destruct (address_eqb_spec (tx_from tx) contract);
+      simpl_goal_invariant;
+      simpl_hyp_invariant;
+      cbn in *; lia.
+  - (* Deployment. Can be deployment of contract, in which case we need to *)
+    (* establish invariant. *)
+    rewrite_environment_equiv.
+    subst new_acts.
+    cbn in congress_deployed.
+    destruct (address_eqb_spec contract to); cycle 1.
+    + (* Deployment of different contract. Holds both if from us or not. *)
+      specialize_hypotheses.
+      destruct (address_eqb_spec (tx_from tx) contract);
+        simpl_goal_invariant;
+        simpl_hyp_invariant;
+        cbn; lia.
+    + (* This is deployment of this contract *)
+      subst to.
+      replace wc with (Congress.contract : WeakContract) in * by congruence.
+      (* State starts at 0 *)
+      erewrite num_cacts_in_state_deployment; [|eassumption].
+      (* Outgoing actions in queue is 0 *)
+      assert (num_outgoing_acts (chain_state_queue prev) contract = 0)
+        as out_acts by eauto;
+        rewrite_queues.
+      simpl_hyp_invariant.
+      (* Outgoing transactions is 0 *)
+      assert (act_from act <> contract)
+        by (eapply undeployed_contract_not_from_self; eauto).
+      simpl_goal_invariant.
+      rewrite undeployed_contract_no_out_txs; auto.
+      cbn; lia.
+  - (* Call. *)
+    rewrite_environment_equiv.
+    specialize_hypotheses.
+    subst new_acts.
+    destruct (address_eqb_spec contract to); cycle 1.
+    + (* Not to contract. Essentially same thing as transfer case above. *)
+      simpl_goal_invariant.
+      rewrite num_outgoing_acts_call_ne; auto.
+      destruct (address_eqb_spec contract from);
+        simpl_goal_invariant;
+        simpl_hyp_invariant;
+        cbn; lia.
+    + (* To contract. This will run code. *)
+      cbn in congress_deployed.
+      replace wc with (Congress.contract : WeakContract) in * by congruence.
+      subst to.
+      match goal with
+      | [H1: wc_receive _ _ _ _ _ = Some _,
+         H2: contract_state _ _ = Some _,
+         H3: tx = build_tx _ _ _ _ |- _] =>
+        generalize (wc_receive_state_well_behaved _ _ _ _ _ _ _ _ _ _ H3 H2 H1)
+      end.
+      destruct (address_eqb_spec contract from);
+        simpl_goal_invariant;
+        simpl_hyp_invariant;
+        intros;
+        rewrite num_outgoing_acts_call;
+        cbn -[add_tx set_contract_state];
+        lia.
+  - match goal with
+    | [H: chain_state_env prev = chain_state_env new |- _] =>
+      rewrite <- H in *
+    end.
+    unfold num_outgoing_acts.
+    match goal with
+    | [Hperm: Permutation _ _ |- _] => rewrite <- Hperm
+    end; auto.
+Qed.
+
+Corollary congress_txs_after_block
+          {ChainBuilder : ChainBuilderType}
+          prev baker acts slot finalization_height new :
+  builder_add_block prev baker acts slot finalization_height = Some new ->
+  forall addr,
+    env_contracts (builder_env new) addr = Some (Congress.contract : WeakContract) ->
+    length (outgoing_txs new addr) <= num_acts_created_in_proposals new addr.
+Proof.
+  intros add_block contract congress_at_addr.
+  pose proof (congress_txs_well_behaved _ _ (builder_trace new) congress_at_addr).
+  cbn in *.
+  lia.
+Qed.
+End Theories.
 End Congress.
-
-(*
-(* This first property states that the Congress will only send out actions
-   to be performed if there is a matching CreateProposal somewhere in the
-   past. That is, no CreateProposal can lead to two batches of actions being
-   sent out, and the actions correspond to the ones passed in CreateProposal. *)
-Theorem congress_no_unmatched_actions
-        (chain : Chain)
-        (
-*)
